## 基础

$$
\begin{aligned}
\left( \mathrm{A}\mathrm{B} \right)^{-1}&=\mathrm{B}^{-1}\mathrm{A}^{-1} \\
\left( \mathrm{A}\mathrm{B}\mathrm{C}\dots \right)^{-1}&=\dots \mathrm{C}^{-1}\mathrm{B}^{-1}\mathrm{A}^{-1} \\
\left( A^{\mathrm{T}} \right)^{-1}&=\left( A^{-1} \right)^{\mathrm{T}} \\
\left( \mathrm{A}+\mathrm{B} \right)^{\mathrm{T}}&=\mathrm{A}^{\mathrm{T}}+\mathrm{B}^{\mathrm{T}}\\
\left( \mathrm{A}\mathrm{B} \right)^{\mathrm{T}}&=\mathrm{B}^{\mathrm{T}}\mathrm{A}^{\mathrm{T}}\\
\left( \mathrm{A}\mathrm{B}\mathrm{C}\dots \right)^{\mathrm{T}}&=\dots \mathrm{C}^{\mathrm{T}}\mathrm{B}^{\mathrm{T}}\mathrm{A}^{\mathrm{T}}\\
\left( A^{\mathrm{H}} \right)^{-1}&=\left( \mathrm{A}^{-1} \right)^{\mathrm{H}}\\
\left( \mathrm{A}+\mathrm{B} \right)^{\mathrm{H}}&=\mathrm{A}^{\mathrm{H}}+\mathrm{B}^{\mathrm{H}}\\
\left( \mathrm{A}\mathrm{B} \right)^{\mathrm{H}}&=\mathrm{B}^{\mathrm{H}}\mathrm{A}^{\mathrm{H}} \\
\left( \mathrm{A}\mathrm{B}\mathrm{C}\dots \right)^{\mathrm{H}}&=\dots \mathrm{C}^{\mathrm{H}}\mathrm{B}^{\mathrm{H}}\mathrm{A}^{\mathrm{H}} 
\end{aligned}
$$

### Trace

$$
\begin{aligned}
\operatorname{trace}\left( \mathrm{A} \right)&=\sum_i A_{i i} \\
\operatorname{trace}\left( \mathrm{A} \right)&=\sum_i \lambda_i,\;\;\;\; \lambda_i = \operatorname{eig}\left( \mathrm{A} \right)\\
\operatorname{trace}\left( \mathrm{A} \right)&=\operatorname{trace}\left( \mathrm{A}^{\mathrm{T}} \right)\\
\operatorname{trace}\left( \mathrm{A}\mathrm{B} \right)&=\operatorname{trace}\left(\mathrm{B}\mathrm{A}  \right)\\
\operatorname{trace}\left( \mathrm{A}+\mathrm{B} \right)&=\operatorname{trace}\left( \mathrm{A} \right)+\operatorname{trace}\left( \mathrm{B} \right) \\
\operatorname{trace}\left( \mathrm{A}\mathrm{B}\mathrm{C} \right)&=\operatorname{trace}\left( \mathrm{B}\mathrm{C}\mathrm{A} \right)=\operatorname{trace}\left( \mathrm{C}\mathrm{A}\mathrm{B} \right)\\
\mathrm{a}^{\mathrm{T}}\mathrm{a}&=\operatorname{trace}\left( \mathrm{a}\mathrm{a}^{\mathrm{T}} \right)
\end{aligned}
$$

### Determinant

Let $\mathrm{A}$ be an $n\times n$ matrix.

$$
\begin{aligned}
\det \left( \mathrm{A} \right)&=\prod_{i} \lambda_i,\;\;\;\;\lambda_i=\operatorname{eig}\left( \mathrm{A} \right)  \\
\det \left( c \mathrm{A} \right)&=c^n \det\left( \mathrm{A} \right),\;\;\;\; \text{if}\;\mathrm{A} \in \mathbb{R}^{n\times n}\\
\det\left( \mathrm{A}^{\mathrm{T}} \right)&=\det\left( \mathrm{A} \right)\\
\det\left( \mathrm{A}\mathrm{B} \right)&=\det\left( \mathrm{A} \right)\det\left( \mathrm{B} \right)\\
\det\left( \mathrm{A}^{-1} \right)&=\frac{1}{\det\left(  \mathrm{A} \right)}\\
\det\left( \mathrm{A}^n \right)&=\det\left( \mathrm{A} \right)^n\\
\det\left( \mathrm{I}+\mathrm{u}\mathrm{v}^{\mathrm{T}} \right)&=1+\mathrm{u}^{\mathrm{T}}\mathrm{v}
\end{aligned}
$$

For $n=2$:

$$
\det\left( \mathrm{I}+\mathrm{A} \right)=1+\det\left( \mathrm{A} \right)+\operatorname{trace}\left( \mathrm{A} \right)
$$

For $n=3$:

$$
\det\left( \mathrm{I}+\mathrm{A} \right)=1+\det\left( \mathrm{A} \right)+\operatorname{trace}\left( \mathrm{A} \right)+\frac{1}{2}\operatorname{trace}\left( \mathrm{A} \right)^2-\frac{1}{2}\operatorname{trace}\left( \mathrm{A}^2 \right)
$$

for $n=4$:

$$
\begin{aligned}
\det\left( \mathrm{I}+\mathrm{A} \right)=1&+\det\left( \mathrm{A} \right)+\operatorname{trace}\left( \mathrm{A} \right)+\frac{1}{2} \\ 
&+\operatorname{trace}\left( \mathrm{A} \right)^2-\frac{1}{2}\operatorname{trace}\left( \mathrm{A}^2 \right)\\
&+\frac{1}{6}\operatorname{trace}\left( \mathrm{A} \right)^3-\frac{1}{2}\operatorname{trace}\left( \mathrm{A} \right)\operatorname{trace}\left( \mathrm{A}^2 \right)+\frac{1}{3}\operatorname{trace}\left( \mathrm{A}^3 \right) \\
\end{aligned}
$$

For smalll $\varepsilon$, the following approximation holds

$$
\det\left( \mathrm{I}+\varepsilon \mathrm{A} \right)\cong 1+\det\left( \mathrm{A} \right)+\varepsilon \operatorname{trace}\left( \mathrm{A} \right)+\frac{1}{2}\varepsilon^2 \operatorname{trace}\left( \mathrm{A} \right)^2-\frac{1}{2}\varepsilon^2\operatorname{trace}\left( \mathrm{A}^2 \right)
$$

### $2\times 2$ 的特例

Consider the matrix $\mathrm{A}$

$$
\mathrm{A}=\begin{bmatrix}
A_{1 1} & A_{12} \\
A_{21} & A_{22} 
\end{bmatrix}
$$

Determinant and trace

$$
\begin{aligned}
\det\left( \mathrm{A} \right)&=A_{11}A_{22}-A_{12}A_{21}\\
\operatorname{trace}\left( \mathrm{A} \right)&=A_{11}+A_{22}
\end{aligned}
$$

Eigenvalues:

$$
\begin{aligned}
\lambda^2-\lambda \cdot \operatorname{trace}\left( \mathrm{A} \right)&+\det\left( \mathrm{A} \right)=0 \\
\lambda_1=\frac{\operatorname{trace}\left( \mathrm{A} \right)+\sqrt{\operatorname{trace}\left( \mathrm{A} \right)^2-4\det\left( \mathrm{A} \right)}}{2}&\;\;\;\;\lambda_2=\frac{\operatorname{trace}\left( \mathrm{A} \right)-\sqrt{\operatorname{trace}\left( \mathrm{A} \right)^2-4\det\left( \mathrm{A} \right)}}{2}\\
\lambda_1+\lambda_2=\operatorname{trace}\left( \mathrm{A} \right)&\;\;\;\;\lambda_1\lambda_2=\det\left( \mathrm{A} \right)
\end{aligned}
$$

Inverse

$$
\mathrm{A}^{-1}=\frac{1}{\det\left( \mathrm{A} \right)}\begin{bmatrix}
A_{22} &-A_{12}  \\
-A_{21} & A_{11} 
\end{bmatrix}
$$

## Derivatives

This section is covering differentiation of a number of expressions with respect to a mateix $\mathrm{X}$. Note that it is always assumed that $\mathrm{X}$ has *no special structure*, i.e. that the elements of $\mathrm{X}$ are independent (e.g. not symmetric, Toeplitz, positive definite). The basic assumptions can be written in a formula as

$$
\frac{\partial X_{kl}}{\partial X_{ij}}=\delta_{ik}\delta_{lj}
$$

this is for e.g vectir forms,

$$
\left[ \frac{\partial \mathrm{x}}{\partial y} \right]_i=\frac{\partial x_i}{\partial y} \;\;\;\;\left[\frac{\partial x}{\partial \mathrm{y}}  \right]_i=\frac{\partial x}{\partial y_i}\;\;\;\;\left[ \frac{\partial \mathrm{x}}{\partial \mathrm{y}} \right]_{ij}=\frac{\partial x_i}{\partial y_j}
$$

> [!NOTE]
>
> 上述公式说明，向量对标量求导和标量对向量求导，逐项求，结果是一个新向量。向量对向量求导，分别从从两个向量中选取两个元素进行求导，然后将求导的结果拼成矩阵即可。

The following rules are general and very useful when deriving the differential of an expression:

$$
\begin{aligned}
\partial \mathrm{A}&=0 \;\;\;\;\left( \mathrm{A}\; \text{is a constant} \right) \\
\partial\left( \alpha \mathrm{X} \right)&=\alpha\partial \mathrm{X} \\
\partial\left( \mathrm{X}+\mathrm{Y} \right)&=\partial \mathrm{X}+\partial \mathrm{Y}\\
\end{aligned}
$$ 



## 特殊矩阵

### Hermitian 矩阵


对于方阵 $\boldsymbol{A} \in \mathbb{C}^{n\times n}$，若 $\boldsymbol{A}=\boldsymbol{A}^{\operatorname{H}}$，即其元素满足 $a_{ij}=a_{ji}^{*}$. 也就是说 Hermitian 是共轭对称矩阵。

显然，如果矩阵式实矩阵，Hermitian 矩阵与对称矩阵等价. 
